[ record ] a bunch of stuff with proof of progress

core+bidir+record/Proof/Application.v
@@ -22,35 +22,83 @@ Require Import LocallyNameless.
 
 (** * Definition *)
 
-Inductive papp : term -> term -> term -> Prop :=
-| Pa_Lit_Tl : forall (A B : type) (v vl : term) (n : nat),
+(** instead of using principal typing to get the type, we can define a function 
+    atype : vl -> arg
+    atype v = Some A
+    atype l = Some l
+ *)
+
+(** value and label *)
+
+Inductive vl : Set :=
+| Av : term -> vl
+| Al : label -> vl.
+
+Hint Constructors vl : core.
+
+(** I'm confused a little bit and try to think why not let merge to be general one (work both on type and label),
+    Since we can't allow label to be merged, so merge case only account for types 
+*)
+
+Inductive atype : vl -> arg -> Prop :=
+| At_Ann : forall e A,
+    atype (Av (Ann e A)) (Avt A)
+| At_Rcd : forall e l A,
+    atype (Av e) (Avt A) ->
+    atype (Av (Fld l e)) (Avt (Rcd l A))
+| At_Mrg : forall e1 e2 A1 A2,
+    atype (Av e1) (Avt A1) ->
+    atype (Av e2) (Avt A2) ->
+    atype (Av (Mrg e1 e2)) (Avt (And A1 A2))
+| At_Lbl : forall l,
+    atype (Al l) (Alt l).
+
+Hint Constructors atype : core.
+
+Inductive papp : term -> vl -> term -> Prop :=
+| Pa_Lit_Tl : forall A B v n,
     toplike B ->
-    papp (Ann (Lit n) (Arr A B)) vl (Ann (Lit 1) B)
-| Pa_Lam_Tl : forall (A B C D : type) (e vl: term),
+    papp (Ann (Lit n) (Arr A B)) (Av v)
+         (Ann (Lit 1) B)
+| Pa_Lit_Tl_R : forall A n l,
+    toplike A ->
+    papp (Ann (Lit n) (Rcd l A)) (Al l)
+         (Ann (Lit 1) A)
+| Pa_Lam_Tl : forall A B C D e v,
     lc (Lam A e B) ->
     toplike D ->
-    papp (Ann (Lam A e B) (Arr C D)) vl
+    papp (Ann (Lam A e B) (Arr C D)) (Av v)
          (Ann (Lit 1) D)
-| Pa_Lam : forall (A B C D : type) (e vl vl' : term),
+| Pa_Lam_Tl_R : forall A B C l e,
     lc (Lam A e B) ->
-    casting vl A vl' ->
+    toplike C ->
+    papp (Ann (Lam A e B) (Rcd l C)) (Al l)
+         (Ann (Lit 1) C)
+| Pa_Lam : forall A B C D v v' e,
+    lc (Lam A e B) ->
+    casting v A v' ->
     not (toplike D) ->
-    papp (Ann (Lam A e B) (Arr C D)) vl
-         (Ann (open e vl') D)
-| Pa_Mrg_L : forall (A B C : type) (v1 v2 vl e: term),
-    ptype v1 A -> ptype v2 B -> ptype vl C ->
-    not (auxas (Some C) B) ->
+    papp (Ann (Lam A e B) (Arr C D)) (Av v)
+         (Ann (open e v') D)
+| Pa_Rcd : forall v l,
+    papp (Fld l v) (Al l) v
+| Pa_Mrg_L : forall v1 v2 A B vl TA e,
+    ptype v1 A -> ptype v2 B ->
+    atype vl TA ->
+    not (auxas (Some TA) B) ->
     papp v1 vl e ->
     papp (Mrg v1 v2) vl e
-| Pa_Mrg_R : forall (A B C : type) (v1 v2 vl e : term),
-    ptype v1 A -> ptype v2 B -> ptype vl C ->
-    not (auxas (Some C) A) ->
+| Pa_Mrg_R : forall v1 v2 A B vl TA e,
+    ptype v1 A -> ptype v2 B ->
+    atype vl TA ->
+    not (auxas (Some TA) A) ->
     papp v2 vl e ->
     papp (Mrg v1 v2) vl e
-| Pa_Mrg_P : forall (A B C : type) (v1 v2 vl e1 e2 : term),
-    ptype v1 A -> ptype v2 B -> ptype vl C ->
-    auxas (Some C) A ->
-    auxas (Some C) B ->
+| Pa_Mrg_P : forall v1 v2 A B vl TA e1 e2,
+    ptype v1 A -> ptype v2 B ->
+    atype vl TA ->
+    auxas (Some TA) A ->
+    auxas (Some TA) B ->
     papp v1 vl e1 ->
     papp v2 vl e2 ->
     papp (Mrg v1 v2) vl (Mrg e1 e2).
@@ -61,6 +109,47 @@ Notation "v · vl ⟹ e" := (papp v vl e) (at level 69).
 
 (** * Determinism *)
 
+Lemma atype_determinism :
+  forall vl TA1 TA2,
+    atype vl TA1 ->
+    atype vl TA2 ->
+    TA1 = TA2.
+Proof.
+  introv At1 At2. gen TA2.
+  dependent induction At1; intros.
+  - dependent destruction At2; eauto.
+  - dependent destruction At2; eauto.
+    pose proof (IHAt1 _ At2) as IH.
+    dependent destruction IH; eauto.
+  - dependent destruction At2.
+    pose proof (IHAt1_1 _ At2_1) as IH1.
+    pose proof (IHAt1_2 _ At2_2) as IH2.
+    dependent destruction IH1. dependent induction IH2.
+    auto.
+  - dependent destruction At2; eauto.
+Qed.
+
+Ltac subst_atype :=
+  match goal with
+  | [H1: atype ?vl ?TA1, H2: atype ?vl ?TA2 |- _] =>
+      (pose proof (atype_determinism _ _ _ H1 H2) as Eqs; subst; clear H2)
+  end.
+
+Lemma typing_to_atype :
+  forall v A,
+    value v ->
+    typing nil v Inf A ->
+    atype (Av v) (Avt A).
+Proof.
+  introv Val Typ. gen A.
+  induction Val; intros.
+  - dependent destruction Typ; eauto.
+  - dependent destruction Typ; eauto.
+  - dependent destruction Typ; eauto.
+Qed.
+
+Hint Resolve typing_to_atype : core.
+
 (** Well-typed application term doesn't ensure that all subterms of function can accept its argument,
     but ensures part of its functions can accept *)
 
@@ -68,396 +157,211 @@ Notation "v · vl ⟹ e" := (papp v vl e) (at level 69).
 
 Section papp_determinism.
 
-Lemma papp_determinism :
-  forall v vl e1 e2 A,
-    value v -> value vl ->
-    papp v vl e1 ->
-    papp v vl e2 ->
-    typing nil (App v vl) Inf A ->
+Ltac solver1 := repeat match goal with
+                       | Typ: typing nil ?v Inf ?A, Val: value ?v, Pt: ptype ?v _ |- _ =>
+                           pose proof (typing_to_ptype _ _ (value_is_uvalue _ Val) Typ);
+                           subst_ptype; clear Pt
+                       | Typ: typing nil ?v Inf ?A, Val: value ?v, At: atype (Av ?v) _ |- _ =>
+                           pose proof (typing_to_atype _ _ Val Typ);
+                           subst_atype; clear At
+                       end;
+                match goal with
+                | As: appsub _ _ _ |- _ => (dependent destruction As; eauto)
+                end.
+
+Lemma papp_determinism_v :
+  forall f v e1 e2 A B C,
+    value f -> value v ->
+    typing nil f Inf A -> typing nil v Inf B ->
+    appsub (Some (Avt B)) A C ->
+    papp f (Av v) e1 ->
+    papp f (Av v) e2 ->
     e1 = e2.
 Proof.
-  Ltac solver1 := repeat match goal with
-                         | [Typ: typing nil ?v Inf ?A, Val: value ?v, Pt: ptype ?v _ |- _] =>
-                             (pose proof (typing_to_ptype _ _ (value_is_uvalue _ Val) Typ); subst_ptype; clear Pt)
-                         end;
-                  match goal with
-                  | [H: appsub _ _ _ |- _] => (dependent destruction H; eauto)
-                  end.  
-  introv Val Vall P1 P2 Typ. gen e2 A.
-  induction P1; intros.
+  introv Valf Val Typ1 Typ2 As P1 P2. gen e2 A B C.
+  dependent induction P1; intros.
   - Case "Lit Toplike".
     dependent destruction P2; eauto.
   - Case "Lam Toplike".
     dependent destruction P2; eauto.
   - Case "Lam".
     dependent destruction P2; eauto.
-    dependent destruction Typ.
     repeat (f_equal). eapply casting_determinism; eauto.
   - Case "Merge L".
-    dependent destruction P2; eauto;
-      repeat subst_ptype; dependent destruction Val;
-      dependent destruction Typ; dependent destruction Typ1; eauto; solver1.
+    dependent destruction P2;
+      repeat subst_ptype; subst_atype;
+      dependent destruction Valf; dependent destruction Typ1; solver1.
   - Case "Merge R".
     dependent destruction P2; eauto;
-      repeat subst_ptype; dependent destruction Val;
-      dependent destruction Typ; dependent destruction Typ1; eauto; solver1.
+      repeat subst_ptype; subst_atype;
+      dependent destruction Valf; dependent destruction Typ1; solver1.
   - Case "Merge P".
     dependent destruction P2; eauto;
-      repeat subst_ptype; dependent destruction Val;
-      dependent destruction Typ; dependent destruction Typ1; eauto.
+      repeat subst_ptype; subst_atype;
+      dependent destruction Valf; dependent destruction Typ1; solver1.
     + f_equal; solver1.
     + f_equal; solver1.
+Qed.
+
+Lemma papp_determinism_l :
+  forall v l e1 e2 A B,
+    value v ->
+    typing nil v Inf A ->
+    appsub (Some (Alt l)) A B ->
+    papp v (Al l) e1 ->
+    papp v (Al l) e2 ->
+    e1 = e2.
+Proof.
+  introv Val Typ As P1 P2. gen e2 A B.
+  dependent induction P1; intros.
+  - Case "Lit Toplike".
+    dependent destruction P2; eauto.
+  - Case "Lam Toplike".
+    dependent destruction P2; eauto.
+  - Case "Prj".
+    dependent destruction P2; eauto.
+  - Case "Mrg L".
+    dependent destruction P2;
+      repeat subst_ptype; subst_atype;
+      match goal with
+      | At: atype (Al _) _ |- _ => dependent destruction At
+      end; eauto;
+      dependent destruction Val; dependent destruction Typ; solver1.
+  - Case "Mrg R".
+    dependent destruction P2;
+      repeat subst_ptype; subst_atype;
+      match goal with
+      | At: atype (Al _) _ |- _ => dependent destruction At
+      end; eauto;
+      dependent destruction Val; dependent destruction Typ; solver1.
+  - Case "Mrg P".
+    dependent destruction P2;
+      repeat subst_ptype; subst_atype;
+      match goal with
+      | At: atype (Al _) _ |- _ => dependent destruction At
+      end; eauto;
+      dependent destruction Val; dependent destruction Typ; solver1.
+    + f_equal; eauto.
+    + f_equal; eauto.
 Qed.
       
 End papp_determinism.
 
 (** * App & Value *)
 
-Lemma papp_lc :
+Lemma papp_lc_v :
   forall v vl e,
     lc v -> lc vl ->
-    papp v vl e ->
+    papp v (Av vl) e ->
     lc e.
 Proof.
   introv Lc Lcl Pa.
   dependent induction Pa; try solve [econstructor; eauto 3].
-  - eapply Lc_Ann. eapply open_abs; eauto.
-    pose proof (casting_lc vl vl' A). eauto 3.
+  - econstructor. eapply open_abs; eauto 3.
+    eapply casting_lc; eauto.
   - dependent destruction Lc; eauto 3.
   - dependent destruction Lc; eauto 3.
 Qed.
 
-(** * App & Consistent *)
-
-(** Automating this lemma is tricky for it has "four" irrelevant cases *)
-
-Section papp_consistent.
-
-Lemma papp_consistent :
-  forall v1 v2 vl e1 e2 A B C,
-    value v1 -> value v2 -> value vl ->
-    typing nil v1 Inf A ->
-    typing nil v2 Inf B ->
-    typing nil vl Inf C ->
-    papp v1 vl e1 ->
-    papp v2 vl e2 ->
-    consistent v1 v2 ->
-    consistent e1 e2.
+Lemma papp_lc_l :
+  forall v vl e,
+    lc v ->
+    papp v (Al vl) e ->
+    lc e.
 Proof.
-  Ltac solver1 := try solve [eapply Con_Dj; eauto; eapply disjoint_toplike; eauto 3].
-  Ltac solver2 := try solve [eapply Con_Dj; eauto; eapply disjoint_symmetry; eapply disjoint_toplike; eauto 3].
-  Ltac solver3 :=  try solve [match goal with
-                              | [Val: value (Mrg ?v1 ?v2),
-                                 Con: consistent _ (Mrg ?v1 ?v2),
-                                 Typ: typing nil (Mrg ?v1 ?v2) Inf _ |- _] =>
-      (dependent destruction Val; eapply consistent_inv_merge_r in Con; destruct Con; dependent destruction Typ; eauto 4)
-                              end].
-  Ltac solver4 :=  try solve [match goal with
-                              | [Val: value (Mrg ?v1 ?v2),
-                                 Con: consistent (Mrg ?v1 ?v2) _,
-                                 Typ: typing nil (Mrg ?v1 ?v2) Inf _ |- _] =>
-      (dependent destruction Val; eapply consistent_inv_merge_l in Con; destruct Con; dependent destruction Typ; eauto 4)
-                              end].
-  introv Val1 Val2 Vall Typ1 Typ2 Typl P1 P2 Con. gen A B C.
-  dependent induction P1.  
-  - Case "Lit-Toplike".
-    dependent induction P2; intros; solver1; solver3.
-  - Case "Lam-Toplike".
-    dependent induction P2; intros; solver1; solver3.
-  - Case "Lam".
-    dependent induction P2; intros; solver2; solver3.
-    dependent destruction Con; eauto.
-    + assert (vl' = vl'0). eapply casting_determinism; eauto. subst. eapply Con_Ann; eauto 4.
-    + assert (vl' = vl'0). eapply casting_determinism; eauto. subst. eapply Con_Ann; eauto 4.
-    + repeat (dependent destruction Typ1; dependent destruction Typ2).
-      repeat match goal with
-               [H: ptype _ _ |- _] => (dependent destruction H)
-             end.
-      eapply Con_Dj; eauto.
-  - Case "Merge L".
-    dependent induction P2; intros; solver4.
-  - Case "Merge R".
-    dependent induction P2; intros; solver4.
-  - Case "Merge P".
-    dependent induction P2; intros; eapply Con_Mrg_L; solver4.
+  introv Lc Pa.
+  dependent induction Pa; try solve [econstructor; eauto 3].
+  - dependent destruction Lc. assumption.
+  - dependent destruction Lc; eauto 3.
+  - dependent destruction Lc; eauto 3.
 Qed.
 
-End papp_consistent.
-
-(** * Weakening Lemma *)
-
-Lemma typing_weakening_gen :
-  forall G E F e A dir,
-    typing (E ++ G) e dir A ->
-    uniq (E ++ F ++ G) ->
-    typing (E ++ F ++ G) e dir A.
-Proof.
-  introv Typ. gen F.
-  dependent induction Typ; introv Env; eauto.
-  pick fresh x and apply Ty_Lam.
-  rewrite_env (([(x,A)] ++ E) ++ F ++ G).
-  apply H0; eauto.
-  solve_uniq.
-Qed.
-
-Lemma typing_weakening :
-  forall E F e A dir,
-    typing E e dir A ->
-    uniq (F ++ E) ->
-    typing (F ++ E) e dir A.
-Proof.
-  intros.
-  rewrite_env (nil ++ F ++ E).
-  eapply typing_weakening_gen; eauto.
-Qed.
-
-(** * Subsitution Lemma *)
-
-Lemma typing_uniq :
-  forall E e T,
-    typing E e Inf T -> uniq E.
-Proof.
-  introv Typ.
-  induction Typ; eauto.
-  - pick fresh x.
-    assert (J: uniq ((one (x,A)) ++ T)); eauto.
-    dependent destruction J; eauto.
-Qed.
-
-Lemma fv_open_lower :
-  forall e1 e2 k,
-    fv e1 [<=] fv (open_rec k e2 e1).
-Proof with auto.
-  intros.
-  generalize dependent k.
-  induction e1; intros; simpl; try fsetdec...
-  - specialize (IHe1_1 k).
-    specialize (IHe1_2 k).
-    fsetdec...
-  - specialize (IHe1_1 k).
-    specialize (IHe1_2 k).
-    fsetdec...
-Qed.
-
-Lemma fv_in_dom :
-  forall T e A dir,
-    typing T e dir A -> fv e [<=] dom T.
-Proof.
-  introv Typ.
-  dependent induction Typ; simpl; try fsetdec; eauto.
-  - apply binds_In in H0.
-    fsetdec.
-  - pick fresh x. 
-    assert ((fv (open e x)) [<=] (dom ((one (x, A)) ++ T))) by eauto.
-    simpl in *.
-    assert (fv e [<=] fv (open e x)).
-    eapply fv_open_lower.
-    assert (fv e [<=] add x (dom T)).
-    fsetdec.
-    eapply add_notin_context; eauto.
-Qed.    
-
-Lemma subst_value :
-  forall e z u A ,
-    typing nil e Inf A -> substitution z u e = e.
-Proof with auto.
-  intros.
-  apply fv_in_dom in H...
-  simpl in H...
-  eapply subst_fresh; eauto.
-  fsetdec.
-Qed.
-
-(** substitution lemma, 
-stating that substituting a (closed, well-typed) term s for a variable x in a term t preserves the type of t *)
-
-Lemma substitution_lemma :
-   forall F E x v e A B C dir,
-    typing (F ++ [(x, A)] ++ E) e dir B ->
-    typing nil v Inf C ->
-    isosub C A ->
-    (exists D, typing (F ++ E) (substitution x v e) dir D /\ isosub D B).
-Proof.
-  introv Typ Typv Isub. remember (F ++ [(x, A)] ++ E) as E'. gen F.
-  induction Typ; intros; simpl; subst; eauto.
-  - Case "Var".
-    destruct (x0 == x); eauto. subst.
-    eapply binds_mid_eq in H0; eauto. subst.
-    exists C. split; eauto.
-    eapply typing_weakening; eauto.
-    rewrite_env (E ++ nil).
-    eapply typing_weakening; eauto.
-    solve_uniq.
-  - Case "Lam".
-    exists (Arr A0 B). split; eauto.
-    eapply (Ty_Lam (union L (singleton x))); eauto. intros.
-    pose proof (H0 x0) as IH.
-    exploit IH; eauto. intros IH'. destruct_conjs.
-    rewrite_env (([(x0, A0)] ++ F) ++ E).
-    rewrite subst_open_var; eauto 3.
-    eapply isosub_to_sub1 in H3.
-    eapply typing_chk_sub; eauto.    
-  - Case "Ann".
-    exists A0. split; eauto.
-    pose proof (IHTyp F) as IH. destruct IH; eauto. destruct_conjs.
-    eapply Ty_Ann; eauto. eapply isosub_to_sub1 in H0.
-    eapply typing_chk_sub; eauto.
-  - Case "App".
-    pose proof (IHTyp1 F) as IH1. pose proof (IHTyp2 F) as IH2.
-    destruct IH1; destruct IH2; eauto. destruct_conjs.
-    eapply appsub_iso in H; eauto. destruct H. destruct H.
-    exists x2. split; eauto.
-  - Case "Merge".
-    pose proof (IHTyp1 F) as IH1. pose proof (IHTyp2 F) as IH2.
-    destruct IH1; destruct IH2; eauto. destruct_conjs.
-    exists (And x0 x1). split; eauto.
-    eapply Ty_Mrg; eauto. eapply disjoint_iso_l; eauto.
-  - Case "Merge V".
-    exists (And A0 B). split; eauto.
-    pose proof (subst_value u1 x v _ Typ1) as Rw1.
-    pose proof (subst_value u2 x v _ Typ2) as Rw2.
-    rewrite Rw1. rewrite Rw2.
-    eapply Ty_Mrg_Uv; eauto.
-  - Case "Sub".
-    pose proof (IHTyp F). destruct H0; eauto. destruct H0.
-    exists B. split; eauto. eapply isosub_to_sub1 in H1.
-    eapply Ty_Sub; eauto. eapply sub_transitivity; eauto.
-Qed.
-
-(** * Preservation *)
-
-Section papp_preservation.
-
-Lemma papp_uvalue :
-  forall v vl e A B,
-    value v -> value vl ->
-    typing nil v Inf A -> typing nil vl Inf B ->
-    papp v vl e ->
-    uvalue e.
-Proof.
-  introv Val Vall Typ Typl Pa. gen A B.
-  induction Pa; intros; eauto 5;
-    try solve [dependent destruction Val; dependent destruction Typ; eauto].
-Qed.  
-
-Lemma papp_preservation :
-  forall v vl e A B C,
-    value v -> value vl ->
-    typing nil v Inf A ->
-    typing nil vl Inf B ->
-    appsub (Some B) A C ->
-    papp v vl e ->
-    (exists D, typing nil e Inf D /\ isosub D C).
-Proof.
-  Ltac solver1 := repeat match goal with
-                         | [Typ: typing nil ?v Inf ?A, Val: value ?v, Pt: ptype ?v _ |- _] =>
-                             (pose proof (typing_to_ptype _ _ (value_is_uvalue _ Val) Typ); subst_ptype; clear Pt)
-                         end.
-  introv Val Vall Typ Typl As Pa. gen A B C.
-  induction Pa; intros.
-  - Case "Lit Toplike".
-    dependent destruction Typ. exists B. split.
-    + eapply Ty_Ann; eauto. eapply typing_chk_sub; eauto.
-      eapply sub_toplike_super; eauto.
-    + dependent destruction As; eauto.
-  - Case "Lam Toplike".
-    dependent destruction Typ. exists D. split.
-    + eapply Ty_Ann; eauto. eapply typing_chk_sub; eauto.
-      eapply sub_toplike_super; eauto.
-    + dependent destruction As; eauto.
-  - Case "Lam".
-    repeat dependent destruction Typ. dependent destruction As.
-    dependent destruction Val.
-    match goal with
-    | [H: sub (Arr _ _) (Arr _ _) |- _] => (dependent destruction H; eauto)
-    end.
-    exists D. split; eauto.
-    match goal with
-    | [H: casting _ _ _ |- _] => (eapply casting_preservation in H; eauto; destruct H; destruct H)
-    end.
-    pick fresh y. rewrite (subst_intro y); eauto.
-    assert (Fr': y `notin` L) by eauto.
-    pose proof (H4 y Fr').
-    rewrite_env (nil ++ [(y, A)] ++ nil) in H8.
-    pose proof (substitution_lemma nil nil y vl' (open e y) A B x Chk) as Sl.
-    destruct Sl as [x' Sl']; eauto. destruct Sl'.
-    eapply Ty_Ann; eauto.
-    eapply isosub_to_sub1 in H10; eauto.
-    eapply typing_chk_sub; eauto.
-    eapply sub_transitivity; eauto 3.
-  - Case "Merge L".
-    dependent destruction Val. dependent destruction Typ;
-      dependent destruction As; eauto 3; solver1; eauto.
-  - Case "Merge R".
-    dependent destruction Val. dependent destruction Typ;
-      dependent destruction As; eauto 3; solver1; eauto.
-  - Case "Merge P".
-    dependent destruction Val. dependent destruction Typ.
-    + solver1.
-      dependent destruction As; eauto.
-      pose proof (IHPa1 Val1 Vall _ Typ1 _ Typl _ As1).
-      pose proof (IHPa2 Val2 Vall _ Typ2 _ Typl _ As2).
-      destruct_conjs. exists (And H H0). split; eauto.
-      eapply Ty_Mrg; eauto.
-      assert (disjoint D1 D2). eapply disjoint_appsub; eauto.
-      eapply disjoint_iso_l; eauto.
-    + solver1.
-      dependent destruction As; eauto.
-      pose proof (IHPa1 Val1 Vall _ Typ1 _ Typl _ As1).
-      pose proof (IHPa2 Val2 Vall _ Typ2 _ Typl _ As2).
-      destruct_conjs. exists (And H H0). split; eauto.
-      pose proof (papp_uvalue _ _ _ _ _ Val1 Vall Typ1 Typl Pa1).
-      pose proof (papp_uvalue _ _ _ _ _ Val2 Vall Typ2 Typl Pa2).
-      eapply Ty_Mrg_Uv; eauto 3.
-      pose proof (papp_consistent v1 v2 vl e1 e2 A0 B0 B1) as Pc.
-      eapply Pc; eauto.    
-Qed.
-
-End papp_preservation.
-    
 (** * Progress *)
 
-Lemma papp_progress :
-  forall v vl A B C,
-    value v -> value vl ->
-    typing nil v Inf A -> typing nil vl Inf B ->
-    appsub (Some B) A C ->
-    exists e, papp v vl e.
+Lemma papp_progress_v :
+  forall f v A B C,
+    value f -> value v ->
+    typing nil f Inf A -> typing nil v Inf B ->
+    appsub (Some (Avt B)) A C ->
+    exists e, papp f (Av v) e.
 Proof.
-  introv Val Vall Typ Typl As. gen A B C vl.
-  induction Val; intros.
+  introv Vf Vv Tf Tv As. gen A B C v.
+  induction Vf; intros.
   - Case "Anno".
     destruct H.
     + SCase "Lit".
-      repeat dependent destruction Typ.
+      repeat dependent destruction Tf.
       dependent destruction H1; eauto. dependent destruction As; eauto.
     + SCase "Lam".
-      repeat dependent destruction Typ.
+      repeat dependent destruction Tf.
       dependent destruction H2; eauto.
       * dependent destruction As; eauto.
       * destruct (toplike_decidable D); eauto.
         dependent destruction As; eauto.
         assert (Sub: sub B1 A1) by (eapply sub_transitivity; eauto).
-        pose proof (casting_progress' _ _ _ Vall Typl Sub) as Ct. destruct Ct.
+        pose proof (casting_progress' _ _ _ Vv Tv Sub) as Ct. destruct Ct.
         eexists. eapply Pa_Lam; eauto.
+  - Case "Rcd".
+    dependent destruction Tf; eauto.
+  - Case "Merge".
+    dependent destruction As.
+    + inversion Tf.
+    + dependent destruction Tf.
+      * pose proof (IHVf1 _ Tf1 _ _ As _ Vv Tv) as IH. destruct IH.
+        eexists. eapply Pa_Mrg_L; eauto.
+      * pose proof (IHVf1 _ Tf1 _ _ As _ Vv Tv) as IH. destruct IH.
+        eexists. eapply Pa_Mrg_L; eauto.
+    + dependent destruction Tf.
+      * pose proof (IHVf2 _ Tf2 _ _ As _ Vv Tv) as IH. destruct IH.
+        eexists. eapply Pa_Mrg_R; eauto.
+      * pose proof (IHVf2 _ Tf2 _ _ As _ Vv Tv) as IH. destruct IH.
+        eexists. eapply Pa_Mrg_R; eauto.
+    + dependent destruction Tf.
+      * pose proof (IHVf1 _ Tf1 _ _ As1 _ Vv Tv) as IH1. destruct IH1.
+        pose proof (IHVf2 _ Tf2 _ _ As2 _ Vv Tv) as IH2. destruct IH2.
+        eexists. eapply Pa_Mrg_P; eauto.
+      * pose proof (IHVf1 _ Tf1 _ _ As1 _ Vv Tv) as IH1. destruct IH1.
+        pose proof (IHVf2 _ Tf2 _ _ As2 _ Vv Tv) as IH2. destruct IH2.
+        eexists. eapply Pa_Mrg_P; eauto.
+Qed.
+
+Lemma papp_progress_l :
+  forall v A B l,
+    value v ->
+    typing nil v Inf A ->
+    appsub (Some (Alt l)) A B ->
+    exists e, papp v (Al l) e.
+Proof.
+  introv Val Typ As. gen A B l.
+  induction Val; intros.
+  - Case "Ann". destruct H.
+    + SCase "Lit".
+      repeat dependent destruction Typ.
+      dependent destruction H1; eauto. dependent destruction As; eauto.
+    + SCase "Lam".
+      repeat dependent destruction Typ.
+      dependent destruction H2; eauto. dependent destruction As; eauto.
+  - Case "Rcd".
+    dependent destruction Typ; eauto.
+    dependent destruction As. eauto.
   - Case "Merge".
     dependent destruction As.
     + inversion Typ.
     + dependent destruction Typ.
-      * pose proof (IHVal1 _ Typ1 _ _ As _ Vall Typl) as IH. destruct IH.
+      * pose proof (IHVal1 _ Typ1 _ _ As) as IH. destruct IH.
         eexists. eapply Pa_Mrg_L; eauto.
-      * pose proof (IHVal1 _ Typ1 _ _ As _ Vall Typl) as IH. destruct IH.
+      * pose proof (IHVal1 _ Typ1 _ _ As) as IH. destruct IH.
         eexists. eapply Pa_Mrg_L; eauto.
     + dependent destruction Typ.
-      * pose proof (IHVal2 _ Typ2 _ _ As _ Vall Typl) as IH. destruct IH.
+      * pose proof (IHVal2 _ Typ2 _ _ As) as IH. destruct IH.
         eexists. eapply Pa_Mrg_R; eauto.
-      * pose proof (IHVal2 _ Typ2 _ _ As _ Vall Typl) as IH. destruct IH.
+      * pose proof (IHVal2 _ Typ2 _ _ As) as IH. destruct IH.
         eexists. eapply Pa_Mrg_R; eauto.
     + dependent destruction Typ.
-      * pose proof (IHVal1 _ Typ1 _ _ As1 _ Vall Typl) as IH1. destruct IH1.
-        pose proof (IHVal2 _ Typ2 _ _ As2 _ Vall Typl) as IH2. destruct IH2.
+      * pose proof (IHVal1 _ Typ1 _ _ As1) as IH1. destruct IH1.
+        pose proof (IHVal2 _ Typ2 _ _ As2) as IH2. destruct IH2.
         eexists. eapply Pa_Mrg_P; eauto.
-      * pose proof (IHVal1 _ Typ1 _ _ As1 _ Vall Typl) as IH1. destruct IH1.
-        pose proof (IHVal2 _ Typ2 _ _ As2 _ Vall Typl) as IH2. destruct IH2.
+      * pose proof (IHVal1 _ Typ1 _ _ As1) as IH1. destruct IH1.
+        pose proof (IHVal2 _ Typ2 _ _ As2) as IH2. destruct IH2.
         eexists. eapply Pa_Mrg_P; eauto.
 Qed.
